QCP_examples/humaneval/spec_logic_rewrite_c_files/C_132_goal.v
@@ -1,0 +1,863 @@
+Require Import Coq.ZArith.ZArith.
+Require Import Coq.Bool.Bool.
+Require Import Coq.Strings.String.
+Require Import Coq.Strings.Ascii.
+Require Import Coq.Lists.List.
+Require Import Coq.Classes.RelationClasses.
+Require Import Coq.Classes.Morphisms.
+Require Import Coq.micromega.Psatz.
+Require Import Coq.Sorting.Permutation.
+From AUXLib Require Import int_auto Axioms Feq Idents ListLib VMap.
+Require Import SetsClass.SetsClass. Import SetsNotation.
+From SimpleC.SL Require Import Mem SeparationLogic.
+Require Import Logic.LogicGenerator.demo932.Interface.
+Local Open Scope Z_scope.
+Local Open Scope sets.
+Local Open Scope string_scope.
+Local Open Scope list.
+Import naive_C_Rules.
+Require Import SimpleC.StdLib.string_lib.
+Require Import coins_132.
+Local Open Scope sac.
+From SimpleC.EE.QCP_demos_LLM Require Import char_array_strategy_goal.
+From SimpleC.EE.QCP_demos_LLM Require Import char_array_strategy_proof.
+From SimpleC.StdLib Require Import string_strategy_goal.
+From SimpleC.StdLib Require Import string_strategy_proof.
+
+(*----- Function is_nested -----*)
+
+Definition is_nested_safety_wit_1 := 
+forall (str_pre: Z) (input: (@list Z)) (retval: Z) (PreH1 : (retval = (string_length (input)))) (PreH2 : (0 <= ((string_length (input)) + 1 ))) (PreH3 : (valid_string input )) (PreH4 : (problem_132_pre_z input )) (PreH5 : (bracket_codes_z_132 input )) (PreH6 : ((string_length (input)) < INT_MAX)) ,
+  ((( &( "count" ) )) # Int  |->_)
+  **  (store_string str_pre input )
+  **  ((( &( "n" ) )) # Int  |-> retval)
+  **  ((( &( "str" ) )) # Ptr  |-> str_pre)
+|--
+  “ (0 <= INT_MAX) ” 
+  &&  “ ((INT_MIN) <= 0) ”
+.
+
+Definition is_nested_safety_wit_2 := 
+forall (str_pre: Z) (input: (@list Z)) (retval: Z) (PreH1 : (retval = (string_length (input)))) (PreH2 : (0 <= ((string_length (input)) + 1 ))) (PreH3 : (valid_string input )) (PreH4 : (problem_132_pre_z input )) (PreH5 : (bracket_codes_z_132 input )) (PreH6 : ((string_length (input)) < INT_MAX)) ,
+  ((( &( "maxcount" ) )) # Int  |->_)
+  **  ((( &( "count" ) )) # Int  |-> 0)
+  **  (store_string str_pre input )
+  **  ((( &( "n" ) )) # Int  |-> retval)
+  **  ((( &( "str" ) )) # Ptr  |-> str_pre)
+|--
+  “ (0 <= INT_MAX) ” 
+  &&  “ ((INT_MIN) <= 0) ”
+.
+
+Definition is_nested_safety_wit_3 := 
+forall (str_pre: Z) (input: (@list Z)) (retval: Z) (PreH1 : (retval = (string_length (input)))) (PreH2 : (0 <= ((string_length (input)) + 1 ))) (PreH3 : (valid_string input )) (PreH4 : (problem_132_pre_z input )) (PreH5 : (bracket_codes_z_132 input )) (PreH6 : ((string_length (input)) < INT_MAX)) ,
+  ((( &( "ch" ) )) # Int  |->_)
+  **  ((( &( "i" ) )) # Int  |->_)
+  **  ((( &( "maxcount" ) )) # Int  |-> 0)
+  **  ((( &( "count" ) )) # Int  |-> 0)
+  **  (store_string str_pre input )
+  **  ((( &( "n" ) )) # Int  |-> retval)
+  **  ((( &( "str" ) )) # Ptr  |-> str_pre)
+|--
+  “ (0 <= INT_MAX) ” 
+  &&  “ ((INT_MIN) <= 0) ”
+.
+
+Definition is_nested_safety_wit_4 := 
+forall (str_pre: Z) (input: (@list Z)) (retval: Z) (PreH1 : (retval = (string_length (input)))) (PreH2 : (0 <= ((string_length (input)) + 1 ))) (PreH3 : (valid_string input )) (PreH4 : (problem_132_pre_z input )) (PreH5 : (bracket_codes_z_132 input )) (PreH6 : ((string_length (input)) < INT_MAX)) ,
+  ((( &( "ch" ) )) # Int  |-> 0)
+  **  ((( &( "i" ) )) # Int  |->_)
+  **  ((( &( "maxcount" ) )) # Int  |-> 0)
+  **  ((( &( "count" ) )) # Int  |-> 0)
+  **  (store_string str_pre input )
+  **  ((( &( "n" ) )) # Int  |-> retval)
+  **  ((( &( "str" ) )) # Ptr  |-> str_pre)
+|--
+  “ (0 <= INT_MAX) ” 
+  &&  “ ((INT_MIN) <= 0) ”
+.
+
+Definition is_nested_safety_wit_5 := 
+forall (str_pre: Z) (input: (@list Z)) (ch: Z) (maxcount: Z) (count: Z) (i: Z) (n: Z) (PreH1 : (i < n)) (PreH2 : (n = (string_length (input)))) (PreH3 : (0 <= i)) (PreH4 : (i <= n)) (PreH5 : (0 <= count)) (PreH6 : (count <= maxcount)) (PreH7 : (maxcount <= i)) (PreH8 : (0 <= ch)) (PreH9 : (ch <= 127)) (PreH10 : (valid_string input )) (PreH11 : (problem_132_pre_z input )) (PreH12 : (bracket_codes_z_132 input )) (PreH13 : ((string_length (input)) < INT_MAX)) (PreH14 : (nested_scan_state_132 input i count maxcount )) ,
+  ((( &( "str" ) )) # Ptr  |-> str_pre)
+  **  ((( &( "n" ) )) # Int  |-> n)
+  **  ((( &( "i" ) )) # Int  |-> i)
+  **  ((( &( "count" ) )) # Int  |-> count)
+  **  ((( &( "maxcount" ) )) # Int  |-> maxcount)
+  **  ((( &( "ch" ) )) # Int  |-> (Znth i (c_string (input)) 0))
+  **  (store_string str_pre input )
+|--
+  “ (91 <= INT_MAX) ” 
+  &&  “ ((INT_MIN) <= 91) ”
+.
+
+Definition is_nested_safety_wit_6 := 
+forall (str_pre: Z) (input: (@list Z)) (ch: Z) (maxcount: Z) (count: Z) (i: Z) (n: Z) (PreH1 : ((Znth i (c_string (input)) 0) = 91)) (PreH2 : (i < n)) (PreH3 : (n = (string_length (input)))) (PreH4 : (0 <= i)) (PreH5 : (i <= n)) (PreH6 : (0 <= count)) (PreH7 : (count <= maxcount)) (PreH8 : (maxcount <= i)) (PreH9 : (0 <= ch)) (PreH10 : (ch <= 127)) (PreH11 : (valid_string input )) (PreH12 : (problem_132_pre_z input )) (PreH13 : (bracket_codes_z_132 input )) (PreH14 : ((string_length (input)) < INT_MAX)) (PreH15 : (nested_scan_state_132 input i count maxcount )) ,
+  ((( &( "str" ) )) # Ptr  |-> str_pre)
+  **  ((( &( "n" ) )) # Int  |-> n)
+  **  ((( &( "i" ) )) # Int  |-> i)
+  **  ((( &( "count" ) )) # Int  |-> count)
+  **  ((( &( "maxcount" ) )) # Int  |-> maxcount)
+  **  ((( &( "ch" ) )) # Int  |-> (Znth i (c_string (input)) 0))
+  **  (store_string str_pre input )
+|--
+  “ ((count + 1 ) <= INT_MAX) ” 
+  &&  “ ((INT_MIN) <= (count + 1 )) ”
+.
+
+Definition is_nested_safety_wit_7 := 
+forall (str_pre: Z) (input: (@list Z)) (ch: Z) (maxcount: Z) (count: Z) (i: Z) (n: Z) (PreH1 : ((Znth i (c_string (input)) 0) = 91)) (PreH2 : (i < n)) (PreH3 : (n = (string_length (input)))) (PreH4 : (0 <= i)) (PreH5 : (i <= n)) (PreH6 : (0 <= count)) (PreH7 : (count <= maxcount)) (PreH8 : (maxcount <= i)) (PreH9 : (0 <= ch)) (PreH10 : (ch <= 127)) (PreH11 : (valid_string input )) (PreH12 : (problem_132_pre_z input )) (PreH13 : (bracket_codes_z_132 input )) (PreH14 : ((string_length (input)) < INT_MAX)) (PreH15 : (nested_scan_state_132 input i count maxcount )) ,
+  ((( &( "str" ) )) # Ptr  |-> str_pre)
+  **  ((( &( "n" ) )) # Int  |-> n)
+  **  ((( &( "i" ) )) # Int  |-> i)
+  **  ((( &( "count" ) )) # Int  |-> count)
+  **  ((( &( "maxcount" ) )) # Int  |-> maxcount)
+  **  ((( &( "ch" ) )) # Int  |-> (Znth i (c_string (input)) 0))
+  **  (store_string str_pre input )
+|--
+  “ (1 <= INT_MAX) ” 
+  &&  “ ((INT_MIN) <= 1) ”
+.
+
+Definition is_nested_safety_wit_8 := 
+forall (str_pre: Z) (input: (@list Z)) (ch: Z) (maxcount: Z) (count: Z) (i: Z) (n: Z) (PreH1 : ((Znth i (c_string (input)) 0) = 91)) (PreH2 : (i < n)) (PreH3 : (n = (string_length (input)))) (PreH4 : (0 <= i)) (PreH5 : (i <= n)) (PreH6 : (0 <= count)) (PreH7 : (count <= maxcount)) (PreH8 : (maxcount <= i)) (PreH9 : (0 <= ch)) (PreH10 : (ch <= 127)) (PreH11 : (valid_string input )) (PreH12 : (problem_132_pre_z input )) (PreH13 : (bracket_codes_z_132 input )) (PreH14 : ((string_length (input)) < INT_MAX)) (PreH15 : (nested_scan_state_132 input i count maxcount )) ,
+  ((( &( "str" ) )) # Ptr  |-> str_pre)
+  **  ((( &( "n" ) )) # Int  |-> n)
+  **  ((( &( "i" ) )) # Int  |-> i)
+  **  ((( &( "count" ) )) # Int  |-> (count + 1 ))
+  **  ((( &( "maxcount" ) )) # Int  |-> maxcount)
+  **  ((( &( "ch" ) )) # Int  |-> (Znth i (c_string (input)) 0))
+  **  (store_string str_pre input )
+|--
+  “ (93 <= INT_MAX) ” 
+  &&  “ ((INT_MIN) <= 93) ”
+.
+
+Definition is_nested_safety_wit_9 := 
+forall (str_pre: Z) (input: (@list Z)) (ch: Z) (maxcount: Z) (count: Z) (i: Z) (n: Z) (PreH1 : ((Znth i (c_string (input)) 0) <> 91)) (PreH2 : (i < n)) (PreH3 : (n = (string_length (input)))) (PreH4 : (0 <= i)) (PreH5 : (i <= n)) (PreH6 : (0 <= count)) (PreH7 : (count <= maxcount)) (PreH8 : (maxcount <= i)) (PreH9 : (0 <= ch)) (PreH10 : (ch <= 127)) (PreH11 : (valid_string input )) (PreH12 : (problem_132_pre_z input )) (PreH13 : (bracket_codes_z_132 input )) (PreH14 : ((string_length (input)) < INT_MAX)) (PreH15 : (nested_scan_state_132 input i count maxcount )) ,
+  ((( &( "str" ) )) # Ptr  |-> str_pre)
+  **  ((( &( "n" ) )) # Int  |-> n)
+  **  ((( &( "i" ) )) # Int  |-> i)
+  **  ((( &( "count" ) )) # Int  |-> count)
+  **  ((( &( "maxcount" ) )) # Int  |-> maxcount)
+  **  ((( &( "ch" ) )) # Int  |-> (Znth i (c_string (input)) 0))
+  **  (store_string str_pre input )
+|--
+  “ (93 <= INT_MAX) ” 
+  &&  “ ((INT_MIN) <= 93) ”
+.
+
+Definition is_nested_safety_wit_10 := 
+forall (str_pre: Z) (input: (@list Z)) (ch: Z) (maxcount: Z) (count: Z) (i: Z) (n: Z) (PreH1 : ((Znth i (c_string (input)) 0) = 93)) (PreH2 : ((Znth i (c_string (input)) 0) = 91)) (PreH3 : (i < n)) (PreH4 : (n = (string_length (input)))) (PreH5 : (0 <= i)) (PreH6 : (i <= n)) (PreH7 : (0 <= count)) (PreH8 : (count <= maxcount)) (PreH9 : (maxcount <= i)) (PreH10 : (0 <= ch)) (PreH11 : (ch <= 127)) (PreH12 : (valid_string input )) (PreH13 : (problem_132_pre_z input )) (PreH14 : (bracket_codes_z_132 input )) (PreH15 : ((string_length (input)) < INT_MAX)) (PreH16 : (nested_scan_state_132 input i count maxcount )) ,
+  ((( &( "str" ) )) # Ptr  |-> str_pre)
+  **  ((( &( "n" ) )) # Int  |-> n)
+  **  ((( &( "i" ) )) # Int  |-> i)
+  **  ((( &( "count" ) )) # Int  |-> (count + 1 ))
+  **  ((( &( "maxcount" ) )) # Int  |-> maxcount)
+  **  ((( &( "ch" ) )) # Int  |-> (Znth i (c_string (input)) 0))
+  **  (store_string str_pre input )
+|--
+  “ False ”
+.
+
+Definition is_nested_safety_wit_11 := 
+forall (str_pre: Z) (input: (@list Z)) (ch: Z) (maxcount: Z) (count: Z) (i: Z) (n: Z) (PreH1 : ((Znth i (c_string (input)) 0) = 93)) (PreH2 : ((Znth i (c_string (input)) 0) <> 91)) (PreH3 : (i < n)) (PreH4 : (n = (string_length (input)))) (PreH5 : (0 <= i)) (PreH6 : (i <= n)) (PreH7 : (0 <= count)) (PreH8 : (count <= maxcount)) (PreH9 : (maxcount <= i)) (PreH10 : (0 <= ch)) (PreH11 : (ch <= 127)) (PreH12 : (valid_string input )) (PreH13 : (problem_132_pre_z input )) (PreH14 : (bracket_codes_z_132 input )) (PreH15 : ((string_length (input)) < INT_MAX)) (PreH16 : (nested_scan_state_132 input i count maxcount )) ,
+  ((( &( "str" ) )) # Ptr  |-> str_pre)
+  **  ((( &( "n" ) )) # Int  |-> n)
+  **  ((( &( "i" ) )) # Int  |-> i)
+  **  ((( &( "count" ) )) # Int  |-> count)
+  **  ((( &( "maxcount" ) )) # Int  |-> maxcount)
+  **  ((( &( "ch" ) )) # Int  |-> (Znth i (c_string (input)) 0))
+  **  (store_string str_pre input )
+|--
+  “ ((count - 1 ) <= INT_MAX) ” 
+  &&  “ ((INT_MIN) <= (count - 1 )) ”
+.
+
+Definition is_nested_safety_wit_12 := 
+forall (str_pre: Z) (input: (@list Z)) (ch: Z) (maxcount: Z) (count: Z) (i: Z) (n: Z) (PreH1 : ((Znth i (c_string (input)) 0) = 93)) (PreH2 : ((Znth i (c_string (input)) 0) <> 91)) (PreH3 : (i < n)) (PreH4 : (n = (string_length (input)))) (PreH5 : (0 <= i)) (PreH6 : (i <= n)) (PreH7 : (0 <= count)) (PreH8 : (count <= maxcount)) (PreH9 : (maxcount <= i)) (PreH10 : (0 <= ch)) (PreH11 : (ch <= 127)) (PreH12 : (valid_string input )) (PreH13 : (problem_132_pre_z input )) (PreH14 : (bracket_codes_z_132 input )) (PreH15 : ((string_length (input)) < INT_MAX)) (PreH16 : (nested_scan_state_132 input i count maxcount )) ,
+  ((( &( "str" ) )) # Ptr  |-> str_pre)
+  **  ((( &( "n" ) )) # Int  |-> n)
+  **  ((( &( "i" ) )) # Int  |-> i)
+  **  ((( &( "count" ) )) # Int  |-> count)
+  **  ((( &( "maxcount" ) )) # Int  |-> maxcount)
+  **  ((( &( "ch" ) )) # Int  |-> (Znth i (c_string (input)) 0))
+  **  (store_string str_pre input )
+|--
+  “ (1 <= INT_MAX) ” 
+  &&  “ ((INT_MIN) <= 1) ”
+.
+
+Definition is_nested_safety_wit_13 := 
+forall (str_pre: Z) (input: (@list Z)) (ch: Z) (maxcount: Z) (count: Z) (i: Z) (n: Z) (PreH1 : ((Znth i (c_string (input)) 0) = 93)) (PreH2 : ((Znth i (c_string (input)) 0) <> 91)) (PreH3 : (i < n)) (PreH4 : (n = (string_length (input)))) (PreH5 : (0 <= i)) (PreH6 : (i <= n)) (PreH7 : (0 <= count)) (PreH8 : (count <= maxcount)) (PreH9 : (maxcount <= i)) (PreH10 : (0 <= ch)) (PreH11 : (ch <= 127)) (PreH12 : (valid_string input )) (PreH13 : (problem_132_pre_z input )) (PreH14 : (bracket_codes_z_132 input )) (PreH15 : ((string_length (input)) < INT_MAX)) (PreH16 : (nested_scan_state_132 input i count maxcount )) ,
+  ((( &( "str" ) )) # Ptr  |-> str_pre)
+  **  ((( &( "n" ) )) # Int  |-> n)
+  **  ((( &( "i" ) )) # Int  |-> i)
+  **  ((( &( "count" ) )) # Int  |-> (count - 1 ))
+  **  ((( &( "maxcount" ) )) # Int  |-> maxcount)
+  **  ((( &( "ch" ) )) # Int  |-> (Znth i (c_string (input)) 0))
+  **  (store_string str_pre input )
+|--
+  “ (0 <= INT_MAX) ” 
+  &&  “ ((INT_MIN) <= 0) ”
+.
+
+Definition is_nested_safety_wit_14 := 
+forall (str_pre: Z) (input: (@list Z)) (ch: Z) (maxcount: Z) (count: Z) (i: Z) (n: Z) (PreH1 : ((Znth i (c_string (input)) 0) <> 93)) (PreH2 : ((Znth i (c_string (input)) 0) = 91)) (PreH3 : (i < n)) (PreH4 : (n = (string_length (input)))) (PreH5 : (0 <= i)) (PreH6 : (i <= n)) (PreH7 : (0 <= count)) (PreH8 : (count <= maxcount)) (PreH9 : (maxcount <= i)) (PreH10 : (0 <= ch)) (PreH11 : (ch <= 127)) (PreH12 : (valid_string input )) (PreH13 : (problem_132_pre_z input )) (PreH14 : (bracket_codes_z_132 input )) (PreH15 : ((string_length (input)) < INT_MAX)) (PreH16 : (nested_scan_state_132 input i count maxcount )) ,
+  ((( &( "str" ) )) # Ptr  |-> str_pre)
+  **  ((( &( "n" ) )) # Int  |-> n)
+  **  ((( &( "i" ) )) # Int  |-> i)
+  **  ((( &( "count" ) )) # Int  |-> (count + 1 ))
+  **  ((( &( "maxcount" ) )) # Int  |-> maxcount)
+  **  ((( &( "ch" ) )) # Int  |-> (Znth i (c_string (input)) 0))
+  **  (store_string str_pre input )
+|--
+  “ (0 <= INT_MAX) ” 
+  &&  “ ((INT_MIN) <= 0) ”
+.
+
+Definition is_nested_safety_wit_15 := 
+forall (str_pre: Z) (input: (@list Z)) (ch: Z) (maxcount: Z) (count: Z) (i: Z) (n: Z) (PreH1 : ((Znth i (c_string (input)) 0) <> 93)) (PreH2 : ((Znth i (c_string (input)) 0) <> 91)) (PreH3 : (i < n)) (PreH4 : (n = (string_length (input)))) (PreH5 : (0 <= i)) (PreH6 : (i <= n)) (PreH7 : (0 <= count)) (PreH8 : (count <= maxcount)) (PreH9 : (maxcount <= i)) (PreH10 : (0 <= ch)) (PreH11 : (ch <= 127)) (PreH12 : (valid_string input )) (PreH13 : (problem_132_pre_z input )) (PreH14 : (bracket_codes_z_132 input )) (PreH15 : ((string_length (input)) < INT_MAX)) (PreH16 : (nested_scan_state_132 input i count maxcount )) ,
+  ((( &( "str" ) )) # Ptr  |-> str_pre)
+  **  ((( &( "n" ) )) # Int  |-> n)
+  **  ((( &( "i" ) )) # Int  |-> i)
+  **  ((( &( "count" ) )) # Int  |-> count)
+  **  ((( &( "maxcount" ) )) # Int  |-> maxcount)
+  **  ((( &( "ch" ) )) # Int  |-> (Znth i (c_string (input)) 0))
+  **  (store_string str_pre input )
+|--
+  “ (0 <= INT_MAX) ” 
+  &&  “ ((INT_MIN) <= 0) ”
+.
+
+Definition is_nested_safety_wit_16 := 
+forall (str_pre: Z) (input: (@list Z)) (ch: Z) (maxcount: Z) (count: Z) (i: Z) (n: Z) (PreH1 : ((count + 1 ) < 0)) (PreH2 : ((Znth i (c_string (input)) 0) <> 93)) (PreH3 : ((Znth i (c_string (input)) 0) = 91)) (PreH4 : (i < n)) (PreH5 : (n = (string_length (input)))) (PreH6 : (0 <= i)) (PreH7 : (i <= n)) (PreH8 : (0 <= count)) (PreH9 : (count <= maxcount)) (PreH10 : (maxcount <= i)) (PreH11 : (0 <= ch)) (PreH12 : (ch <= 127)) (PreH13 : (valid_string input )) (PreH14 : (problem_132_pre_z input )) (PreH15 : (bracket_codes_z_132 input )) (PreH16 : ((string_length (input)) < INT_MAX)) (PreH17 : (nested_scan_state_132 input i count maxcount )) ,
+  ((( &( "str" ) )) # Ptr  |-> str_pre)
+  **  ((( &( "n" ) )) # Int  |-> n)
+  **  ((( &( "i" ) )) # Int  |-> i)
+  **  ((( &( "count" ) )) # Int  |-> (count + 1 ))
+  **  ((( &( "maxcount" ) )) # Int  |-> maxcount)
+  **  ((( &( "ch" ) )) # Int  |-> (Znth i (c_string (input)) 0))
+  **  (store_string str_pre input )
+|--
+  “ False ”
+.
+
+Definition is_nested_safety_wit_17 := 
+forall (str_pre: Z) (input: (@list Z)) (ch: Z) (maxcount: Z) (count: Z) (i: Z) (n: Z) (PreH1 : (count < 0)) (PreH2 : ((Znth i (c_string (input)) 0) <> 93)) (PreH3 : ((Znth i (c_string (input)) 0) <> 91)) (PreH4 : (i < n)) (PreH5 : (n = (string_length (input)))) (PreH6 : (0 <= i)) (PreH7 : (i <= n)) (PreH8 : (0 <= count)) (PreH9 : (count <= maxcount)) (PreH10 : (maxcount <= i)) (PreH11 : (0 <= ch)) (PreH12 : (ch <= 127)) (PreH13 : (valid_string input )) (PreH14 : (problem_132_pre_z input )) (PreH15 : (bracket_codes_z_132 input )) (PreH16 : ((string_length (input)) < INT_MAX)) (PreH17 : (nested_scan_state_132 input i count maxcount )) ,
+  ((( &( "str" ) )) # Ptr  |-> str_pre)
+  **  ((( &( "n" ) )) # Int  |-> n)
+  **  ((( &( "i" ) )) # Int  |-> i)
+  **  ((( &( "count" ) )) # Int  |-> count)
+  **  ((( &( "maxcount" ) )) # Int  |-> maxcount)
+  **  ((( &( "ch" ) )) # Int  |-> (Znth i (c_string (input)) 0))
+  **  (store_string str_pre input )
+|--
+  “ False ”
+.
+
+Definition is_nested_safety_wit_18 := 
+forall (str_pre: Z) (input: (@list Z)) (ch: Z) (maxcount: Z) (count: Z) (i: Z) (n: Z) (PreH1 : ((count - 1 ) < 0)) (PreH2 : ((Znth i (c_string (input)) 0) = 93)) (PreH3 : ((Znth i (c_string (input)) 0) <> 91)) (PreH4 : (i < n)) (PreH5 : (n = (string_length (input)))) (PreH6 : (0 <= i)) (PreH7 : (i <= n)) (PreH8 : (0 <= count)) (PreH9 : (count <= maxcount)) (PreH10 : (maxcount <= i)) (PreH11 : (0 <= ch)) (PreH12 : (ch <= 127)) (PreH13 : (valid_string input )) (PreH14 : (problem_132_pre_z input )) (PreH15 : (bracket_codes_z_132 input )) (PreH16 : ((string_length (input)) < INT_MAX)) (PreH17 : (nested_scan_state_132 input i count maxcount )) ,
+  ((( &( "str" ) )) # Ptr  |-> str_pre)
+  **  ((( &( "n" ) )) # Int  |-> n)
+  **  ((( &( "i" ) )) # Int  |-> i)
+  **  ((( &( "count" ) )) # Int  |-> (count - 1 ))
+  **  ((( &( "maxcount" ) )) # Int  |-> maxcount)
+  **  ((( &( "ch" ) )) # Int  |-> (Znth i (c_string (input)) 0))
+  **  (store_string str_pre input )
+|--
+  “ (0 <= INT_MAX) ” 
+  &&  “ ((INT_MIN) <= 0) ”
+.
+
+Definition is_nested_safety_wit_19 := 
+forall (str_pre: Z) (input: (@list Z)) (ch: Z) (maxcount: Z) (count: Z) (i: Z) (n: Z) (PreH1 : (0 > maxcount)) (PreH2 : ((count - 1 ) < 0)) (PreH3 : ((Znth i (c_string (input)) 0) = 93)) (PreH4 : ((Znth i (c_string (input)) 0) <> 91)) (PreH5 : (i < n)) (PreH6 : (n = (string_length (input)))) (PreH7 : (0 <= i)) (PreH8 : (i <= n)) (PreH9 : (0 <= count)) (PreH10 : (count <= maxcount)) (PreH11 : (maxcount <= i)) (PreH12 : (0 <= ch)) (PreH13 : (ch <= 127)) (PreH14 : (valid_string input )) (PreH15 : (problem_132_pre_z input )) (PreH16 : (bracket_codes_z_132 input )) (PreH17 : ((string_length (input)) < INT_MAX)) (PreH18 : (nested_scan_state_132 input i count maxcount )) ,
+  ((( &( "str" ) )) # Ptr  |-> str_pre)
+  **  ((( &( "n" ) )) # Int  |-> n)
+  **  ((( &( "i" ) )) # Int  |-> i)
+  **  ((( &( "count" ) )) # Int  |-> 0)
+  **  ((( &( "maxcount" ) )) # Int  |-> maxcount)
+  **  ((( &( "ch" ) )) # Int  |-> (Znth i (c_string (input)) 0))
+  **  (store_string str_pre input )
+|--
+  “ False ”
+.
+
+Definition is_nested_safety_wit_20 := 
+forall (str_pre: Z) (input: (@list Z)) (ch: Z) (maxcount: Z) (count: Z) (i: Z) (n: Z) (PreH1 : ((count - 1 ) > maxcount)) (PreH2 : ((count - 1 ) >= 0)) (PreH3 : ((Znth i (c_string (input)) 0) = 93)) (PreH4 : ((Znth i (c_string (input)) 0) <> 91)) (PreH5 : (i < n)) (PreH6 : (n = (string_length (input)))) (PreH7 : (0 <= i)) (PreH8 : (i <= n)) (PreH9 : (0 <= count)) (PreH10 : (count <= maxcount)) (PreH11 : (maxcount <= i)) (PreH12 : (0 <= ch)) (PreH13 : (ch <= 127)) (PreH14 : (valid_string input )) (PreH15 : (problem_132_pre_z input )) (PreH16 : (bracket_codes_z_132 input )) (PreH17 : ((string_length (input)) < INT_MAX)) (PreH18 : (nested_scan_state_132 input i count maxcount )) ,
+  ((( &( "str" ) )) # Ptr  |-> str_pre)
+  **  ((( &( "n" ) )) # Int  |-> n)
+  **  ((( &( "i" ) )) # Int  |-> i)
+  **  ((( &( "count" ) )) # Int  |-> (count - 1 ))
+  **  ((( &( "maxcount" ) )) # Int  |-> maxcount)
+  **  ((( &( "ch" ) )) # Int  |-> (Znth i (c_string (input)) 0))
+  **  (store_string str_pre input )
+|--
+  “ False ”
+.
+
+Definition is_nested_safety_wit_21 := 
+forall (str_pre: Z) (input: (@list Z)) (ch: Z) (maxcount: Z) (count: Z) (i: Z) (n: Z) (PreH1 : (count > maxcount)) (PreH2 : (count >= 0)) (PreH3 : ((Znth i (c_string (input)) 0) <> 93)) (PreH4 : ((Znth i (c_string (input)) 0) <> 91)) (PreH5 : (i < n)) (PreH6 : (n = (string_length (input)))) (PreH7 : (0 <= i)) (PreH8 : (i <= n)) (PreH9 : (0 <= count)) (PreH10 : (count <= maxcount)) (PreH11 : (maxcount <= i)) (PreH12 : (0 <= ch)) (PreH13 : (ch <= 127)) (PreH14 : (valid_string input )) (PreH15 : (problem_132_pre_z input )) (PreH16 : (bracket_codes_z_132 input )) (PreH17 : ((string_length (input)) < INT_MAX)) (PreH18 : (nested_scan_state_132 input i count maxcount )) ,
+  ((( &( "str" ) )) # Ptr  |-> str_pre)
+  **  ((( &( "n" ) )) # Int  |-> n)
+  **  ((( &( "i" ) )) # Int  |-> i)
+  **  ((( &( "count" ) )) # Int  |-> count)
+  **  ((( &( "maxcount" ) )) # Int  |-> maxcount)
+  **  ((( &( "ch" ) )) # Int  |-> (Znth i (c_string (input)) 0))
+  **  (store_string str_pre input )
+|--
+  “ False ”
+.
+
+Definition is_nested_safety_wit_22 := 
+forall (str_pre: Z) (input: (@list Z)) (n: Z) (i: Z) (count: Z) (maxcount: Z) (ch: Z) (PreH1 : (n = (string_length (input)))) (PreH2 : (0 <= i)) (PreH3 : (i < n)) (PreH4 : (0 <= count)) (PreH5 : (count <= maxcount)) (PreH6 : (maxcount <= (i + 1 ))) (PreH7 : (ch = 91)) (PreH8 : (valid_string input )) (PreH9 : (problem_132_pre_z input )) (PreH10 : (bracket_codes_z_132 input )) (PreH11 : ((string_length (input)) < INT_MAX)) (PreH12 : (nested_scan_after_132 input (i + 1 ) count maxcount )) ,
+  ((( &( "str" ) )) # Ptr  |-> str_pre)
+  **  ((( &( "n" ) )) # Int  |-> n)
+  **  ((( &( "i" ) )) # Int  |-> i)
+  **  ((( &( "count" ) )) # Int  |-> count)
+  **  ((( &( "maxcount" ) )) # Int  |-> maxcount)
+  **  ((( &( "ch" ) )) # Int  |-> ch)
+  **  (store_string str_pre input )
+|--
+  “ ((maxcount - 2 ) <= INT_MAX) ” 
+  &&  “ ((INT_MIN) <= (maxcount - 2 )) ”
+.
+
+Definition is_nested_safety_wit_23 := 
+forall (str_pre: Z) (input: (@list Z)) (n: Z) (i: Z) (count: Z) (maxcount: Z) (ch: Z) (PreH1 : (n = (string_length (input)))) (PreH2 : (0 <= i)) (PreH3 : (i < n)) (PreH4 : (0 <= count)) (PreH5 : (count <= maxcount)) (PreH6 : (maxcount <= (i + 1 ))) (PreH7 : (ch = 93)) (PreH8 : (valid_string input )) (PreH9 : (problem_132_pre_z input )) (PreH10 : (bracket_codes_z_132 input )) (PreH11 : ((string_length (input)) < INT_MAX)) (PreH12 : (nested_scan_after_132 input (i + 1 ) count maxcount )) ,
+  ((( &( "str" ) )) # Ptr  |-> str_pre)
+  **  ((( &( "n" ) )) # Int  |-> n)
+  **  ((( &( "i" ) )) # Int  |-> i)
+  **  ((( &( "count" ) )) # Int  |-> count)
+  **  ((( &( "maxcount" ) )) # Int  |-> maxcount)
+  **  ((( &( "ch" ) )) # Int  |-> ch)
+  **  (store_string str_pre input )
+|--
+  “ ((maxcount - 2 ) <= INT_MAX) ” 
+  &&  “ ((INT_MIN) <= (maxcount - 2 )) ”
+.
+
+Definition is_nested_safety_wit_24 := 
+forall (str_pre: Z) (input: (@list Z)) (n: Z) (i: Z) (count: Z) (maxcount: Z) (ch: Z) (PreH1 : (n = (string_length (input)))) (PreH2 : (0 <= i)) (PreH3 : (i < n)) (PreH4 : (0 <= count)) (PreH5 : (count <= maxcount)) (PreH6 : (maxcount <= (i + 1 ))) (PreH7 : (ch = 93)) (PreH8 : (valid_string input )) (PreH9 : (problem_132_pre_z input )) (PreH10 : (bracket_codes_z_132 input )) (PreH11 : ((string_length (input)) < INT_MAX)) (PreH12 : (nested_scan_after_132 input (i + 1 ) count maxcount )) ,
+  ((( &( "str" ) )) # Ptr  |-> str_pre)
+  **  ((( &( "n" ) )) # Int  |-> n)
+  **  ((( &( "i" ) )) # Int  |-> i)
+  **  ((( &( "count" ) )) # Int  |-> count)
+  **  ((( &( "maxcount" ) )) # Int  |-> maxcount)
+  **  ((( &( "ch" ) )) # Int  |-> ch)
+  **  (store_string str_pre input )
+|--
+  “ (2 <= INT_MAX) ” 
+  &&  “ ((INT_MIN) <= 2) ”
+.
+
+Definition is_nested_safety_wit_25 := 
+forall (str_pre: Z) (input: (@list Z)) (n: Z) (i: Z) (count: Z) (maxcount: Z) (ch: Z) (PreH1 : (n = (string_length (input)))) (PreH2 : (0 <= i)) (PreH3 : (i < n)) (PreH4 : (0 <= count)) (PreH5 : (count <= maxcount)) (PreH6 : (maxcount <= (i + 1 ))) (PreH7 : (ch = 91)) (PreH8 : (valid_string input )) (PreH9 : (problem_132_pre_z input )) (PreH10 : (bracket_codes_z_132 input )) (PreH11 : ((string_length (input)) < INT_MAX)) (PreH12 : (nested_scan_after_132 input (i + 1 ) count maxcount )) ,
+  ((( &( "str" ) )) # Ptr  |-> str_pre)
+  **  ((( &( "n" ) )) # Int  |-> n)
+  **  ((( &( "i" ) )) # Int  |-> i)
+  **  ((( &( "count" ) )) # Int  |-> count)
+  **  ((( &( "maxcount" ) )) # Int  |-> maxcount)
+  **  ((( &( "ch" ) )) # Int  |-> ch)
+  **  (store_string str_pre input )
+|--
+  “ (2 <= INT_MAX) ” 
+  &&  “ ((INT_MIN) <= 2) ”
+.
+
+Definition is_nested_safety_wit_26 := 
+forall (str_pre: Z) (input: (@list Z)) (n_addr_v: Z) (count_addr_v: Z) (maxcount_addr_v: Z) (i_addr_v: Z) (ch_addr_v: Z) (PreH1 : (problem_132_result_z input 1 )) ,
+  (store_string str_pre input )
+  **  ((( &( "str" ) )) # Ptr  |-> str_pre)
+  **  ((( &( "n" ) )) # Int  |-> n_addr_v)
+  **  ((( &( "count" ) )) # Int  |-> count_addr_v)
+  **  ((( &( "maxcount" ) )) # Int  |-> maxcount_addr_v)
+  **  ((( &( "i" ) )) # Int  |-> i_addr_v)
+  **  ((( &( "ch" ) )) # Int  |-> ch_addr_v)
+|--
+  “ (1 <= INT_MAX) ” 
+  &&  “ ((INT_MIN) <= 1) ”
+.
+
+Definition is_nested_safety_wit_27 := 
+forall (str_pre: Z) (input: (@list Z)) (n: Z) (i: Z) (count: Z) (maxcount: Z) (ch: Z) (PreH1 : (count > (maxcount - 2 ))) (PreH2 : (n = (string_length (input)))) (PreH3 : (0 <= i)) (PreH4 : (i < n)) (PreH5 : (0 <= count)) (PreH6 : (count <= maxcount)) (PreH7 : (maxcount <= (i + 1 ))) (PreH8 : (ch = 93)) (PreH9 : (valid_string input )) (PreH10 : (problem_132_pre_z input )) (PreH11 : (bracket_codes_z_132 input )) (PreH12 : ((string_length (input)) < INT_MAX)) (PreH13 : (nested_scan_after_132 input (i + 1 ) count maxcount )) ,
+  ((( &( "str" ) )) # Ptr  |-> str_pre)
+  **  ((( &( "n" ) )) # Int  |-> n)
+  **  ((( &( "i" ) )) # Int  |-> i)
+  **  ((( &( "count" ) )) # Int  |-> count)
+  **  ((( &( "maxcount" ) )) # Int  |-> maxcount)
+  **  ((( &( "ch" ) )) # Int  |-> ch)
+  **  (store_string str_pre input )
+|--
+  “ ((i + 1 ) <= INT_MAX) ” 
+  &&  “ ((INT_MIN) <= (i + 1 )) ”
+.
+
+Definition is_nested_safety_wit_28 := 
+forall (str_pre: Z) (input: (@list Z)) (n: Z) (i: Z) (count: Z) (maxcount: Z) (ch: Z) (PreH1 : (count > (maxcount - 2 ))) (PreH2 : (n = (string_length (input)))) (PreH3 : (0 <= i)) (PreH4 : (i < n)) (PreH5 : (0 <= count)) (PreH6 : (count <= maxcount)) (PreH7 : (maxcount <= (i + 1 ))) (PreH8 : (ch = 91)) (PreH9 : (valid_string input )) (PreH10 : (problem_132_pre_z input )) (PreH11 : (bracket_codes_z_132 input )) (PreH12 : ((string_length (input)) < INT_MAX)) (PreH13 : (nested_scan_after_132 input (i + 1 ) count maxcount )) ,
+  ((( &( "str" ) )) # Ptr  |-> str_pre)
+  **  ((( &( "n" ) )) # Int  |-> n)
+  **  ((( &( "i" ) )) # Int  |-> i)
+  **  ((( &( "count" ) )) # Int  |-> count)
+  **  ((( &( "maxcount" ) )) # Int  |-> maxcount)
+  **  ((( &( "ch" ) )) # Int  |-> ch)
+  **  (store_string str_pre input )
+|--
+  “ ((i + 1 ) <= INT_MAX) ” 
+  &&  “ ((INT_MIN) <= (i + 1 )) ”
+.
+
+Definition is_nested_safety_wit_29 := 
+forall (str_pre: Z) (input: (@list Z)) (n_addr_v: Z) (count_addr_v: Z) (maxcount_addr_v: Z) (i_addr_v: Z) (ch_addr_v: Z) (PreH1 : (problem_132_result_z input 0 )) ,
+  (store_string str_pre input )
+  **  ((( &( "str" ) )) # Ptr  |-> str_pre)
+  **  ((( &( "n" ) )) # Int  |-> n_addr_v)
+  **  ((( &( "count" ) )) # Int  |-> count_addr_v)
+  **  ((( &( "maxcount" ) )) # Int  |-> maxcount_addr_v)
+  **  ((( &( "i" ) )) # Int  |-> i_addr_v)
+  **  ((( &( "ch" ) )) # Int  |-> ch_addr_v)
+|--
+  “ (0 <= INT_MAX) ” 
+  &&  “ ((INT_MIN) <= 0) ”
+.
+
+Definition is_nested_entail_wit_1 := 
+(
+forall (str_pre: Z) (input: (@list Z)) (retval: Z) (PreH1 : (retval = (string_length (input)))) (PreH2 : (0 <= ((string_length (input)) + 1 ))) (PreH3 : (valid_string input )) (PreH4 : (problem_132_pre_z input )) (PreH5 : (bracket_codes_z_132 input )) (PreH6 : ((string_length (input)) < INT_MAX)) ,
+  (store_string str_pre input )
+|--
+  “ (retval = (string_length (input))) ” 
+  &&  “ (0 <= 0) ” 
+  &&  “ (0 <= retval) ” 
+  &&  “ (0 <= 0) ” 
+  &&  “ (0 <= 0) ” 
+  &&  “ (0 <= 0) ” 
+  &&  “ (0 <= 0) ” 
+  &&  “ (0 <= 127) ” 
+  &&  “ (valid_string input ) ” 
+  &&  “ (problem_132_pre_z input ) ” 
+  &&  “ (bracket_codes_z_132 input ) ” 
+  &&  “ ((string_length (input)) < INT_MAX) ” 
+  &&  “ (nested_scan_state_132 input 0 0 0 ) ”
+  &&  (store_string str_pre input )
+) \/
+(
+forall (input: (@list Z)) (retval: Z) (PreH1 : (retval = (string_length (input)))) (PreH2 : (0 <= ((string_length (input)) + 1 ))) (PreH3 : (valid_string input )) (PreH4 : (problem_132_pre_z input )) (PreH5 : (bracket_codes_z_132 input )) (PreH6 : ((string_length (input)) < INT_MAX)) ,
+  TT && emp 
+|--
+  “ (nested_scan_state_132 input 0 0 0 ) ” 
+  &&  “ (0 <= retval) ”
+  &&  emp
+).
+
+Definition is_nested_entail_wit_1_split_goal_1 := 
+forall (input: (@list Z)) (retval: Z) (PreH1 : (retval = (string_length (input)))) (PreH2 : (0 <= ((string_length (input)) + 1 ))) (PreH3 : (valid_string input )) (PreH4 : (problem_132_pre_z input )) (PreH5 : (bracket_codes_z_132 input )) (PreH6 : ((string_length (input)) < INT_MAX)) ,
+  TT && emp 
+|--
+  “ (nested_scan_state_132 input 0 0 0 ) ”
+.
+
+Definition is_nested_entail_wit_1_split_goal_2 := 
+forall (input: (@list Z)) (retval: Z) (PreH1 : (retval = (string_length (input)))) (PreH2 : (0 <= ((string_length (input)) + 1 ))) (PreH3 : (valid_string input )) (PreH4 : (problem_132_pre_z input )) (PreH5 : (bracket_codes_z_132 input )) (PreH6 : ((string_length (input)) < INT_MAX)) ,
+  TT && emp 
+|--
+  “ (0 <= retval) ”
+.
+
+Definition is_nested_entail_wit_2_1 := 
+forall (str_pre: Z) (input: (@list Z)) (ch: Z) (maxcount: Z) (count: Z) (i: Z) (n: Z) (PreH1 : (count <= maxcount)) (PreH2 : (count >= 0)) (PreH3 : ((Znth i (c_string (input)) 0) <> 93)) (PreH4 : ((Znth i (c_string (input)) 0) <> 91)) (PreH5 : (i < n)) (PreH6 : (n = (string_length (input)))) (PreH7 : (0 <= i)) (PreH8 : (i <= n)) (PreH9 : (0 <= count)) (PreH10 : (count <= maxcount)) (PreH11 : (maxcount <= i)) (PreH12 : (0 <= ch)) (PreH13 : (ch <= 127)) (PreH14 : (valid_string input )) (PreH15 : (problem_132_pre_z input )) (PreH16 : (bracket_codes_z_132 input )) (PreH17 : ((string_length (input)) < INT_MAX)) (PreH18 : (nested_scan_state_132 input i count maxcount )) ,
+  (store_string str_pre input )
+|--
+  (“ (n = (string_length (input))) ” 
+  &&  “ (0 <= i) ” 
+  &&  “ (i < n) ” 
+  &&  “ (0 <= count) ” 
+  &&  “ (count <= maxcount) ” 
+  &&  “ (maxcount <= (i + 1 )) ” 
+  &&  “ ((Znth i (c_string (input)) 0) = 93) ” 
+  &&  “ (valid_string input ) ” 
+  &&  “ (problem_132_pre_z input ) ” 
+  &&  “ (bracket_codes_z_132 input ) ” 
+  &&  “ ((string_length (input)) < INT_MAX) ” 
+  &&  “ (nested_scan_after_132 input (i + 1 ) count maxcount ) ”
+  &&  (store_string str_pre input ))
+  ||
+  (“ (n = (string_length (input))) ” 
+  &&  “ (0 <= i) ” 
+  &&  “ (i < n) ” 
+  &&  “ (0 <= count) ” 
+  &&  “ (count <= maxcount) ” 
+  &&  “ (maxcount <= (i + 1 )) ” 
+  &&  “ ((Znth i (c_string (input)) 0) = 91) ” 
+  &&  “ (valid_string input ) ” 
+  &&  “ (problem_132_pre_z input ) ” 
+  &&  “ (bracket_codes_z_132 input ) ” 
+  &&  “ ((string_length (input)) < INT_MAX) ” 
+  &&  “ (nested_scan_after_132 input (i + 1 ) count maxcount ) ”
+  &&  (store_string str_pre input ))
+.
+
+Definition is_nested_entail_wit_2_2 := 
+forall (str_pre: Z) (input: (@list Z)) (ch: Z) (maxcount: Z) (count: Z) (i: Z) (n: Z) (PreH1 : ((count + 1 ) <= maxcount)) (PreH2 : ((count + 1 ) >= 0)) (PreH3 : ((Znth i (c_string (input)) 0) <> 93)) (PreH4 : ((Znth i (c_string (input)) 0) = 91)) (PreH5 : (i < n)) (PreH6 : (n = (string_length (input)))) (PreH7 : (0 <= i)) (PreH8 : (i <= n)) (PreH9 : (0 <= count)) (PreH10 : (count <= maxcount)) (PreH11 : (maxcount <= i)) (PreH12 : (0 <= ch)) (PreH13 : (ch <= 127)) (PreH14 : (valid_string input )) (PreH15 : (problem_132_pre_z input )) (PreH16 : (bracket_codes_z_132 input )) (PreH17 : ((string_length (input)) < INT_MAX)) (PreH18 : (nested_scan_state_132 input i count maxcount )) ,
+  (store_string str_pre input )
+|--
+  (“ (n = (string_length (input))) ” 
+  &&  “ (0 <= i) ” 
+  &&  “ (i < n) ” 
+  &&  “ (0 <= (count + 1 )) ” 
+  &&  “ ((count + 1 ) <= maxcount) ” 
+  &&  “ (maxcount <= (i + 1 )) ” 
+  &&  “ ((Znth i (c_string (input)) 0) = 93) ” 
+  &&  “ (valid_string input ) ” 
+  &&  “ (problem_132_pre_z input ) ” 
+  &&  “ (bracket_codes_z_132 input ) ” 
+  &&  “ ((string_length (input)) < INT_MAX) ” 
+  &&  “ (nested_scan_after_132 input (i + 1 ) (count + 1 ) maxcount ) ”
+  &&  (store_string str_pre input ))
+  ||
+  (“ (n = (string_length (input))) ” 
+  &&  “ (0 <= i) ” 
+  &&  “ (i < n) ” 
+  &&  “ (0 <= (count + 1 )) ” 
+  &&  “ ((count + 1 ) <= maxcount) ” 
+  &&  “ (maxcount <= (i + 1 )) ” 
+  &&  “ ((Znth i (c_string (input)) 0) = 91) ” 
+  &&  “ (valid_string input ) ” 
+  &&  “ (problem_132_pre_z input ) ” 
+  &&  “ (bracket_codes_z_132 input ) ” 
+  &&  “ ((string_length (input)) < INT_MAX) ” 
+  &&  “ (nested_scan_after_132 input (i + 1 ) (count + 1 ) maxcount ) ”
+  &&  (store_string str_pre input ))
+.
+
+Definition is_nested_entail_wit_2_3 := 
+forall (str_pre: Z) (input: (@list Z)) (ch: Z) (maxcount: Z) (count: Z) (i: Z) (n: Z) (PreH1 : ((count - 1 ) <= maxcount)) (PreH2 : ((count - 1 ) >= 0)) (PreH3 : ((Znth i (c_string (input)) 0) = 93)) (PreH4 : ((Znth i (c_string (input)) 0) <> 91)) (PreH5 : (i < n)) (PreH6 : (n = (string_length (input)))) (PreH7 : (0 <= i)) (PreH8 : (i <= n)) (PreH9 : (0 <= count)) (PreH10 : (count <= maxcount)) (PreH11 : (maxcount <= i)) (PreH12 : (0 <= ch)) (PreH13 : (ch <= 127)) (PreH14 : (valid_string input )) (PreH15 : (problem_132_pre_z input )) (PreH16 : (bracket_codes_z_132 input )) (PreH17 : ((string_length (input)) < INT_MAX)) (PreH18 : (nested_scan_state_132 input i count maxcount )) ,
+  (store_string str_pre input )
+|--
+  (“ (n = (string_length (input))) ” 
+  &&  “ (0 <= i) ” 
+  &&  “ (i < n) ” 
+  &&  “ (0 <= (count - 1 )) ” 
+  &&  “ ((count - 1 ) <= maxcount) ” 
+  &&  “ (maxcount <= (i + 1 )) ” 
+  &&  “ ((Znth i (c_string (input)) 0) = 93) ” 
+  &&  “ (valid_string input ) ” 
+  &&  “ (problem_132_pre_z input ) ” 
+  &&  “ (bracket_codes_z_132 input ) ” 
+  &&  “ ((string_length (input)) < INT_MAX) ” 
+  &&  “ (nested_scan_after_132 input (i + 1 ) (count - 1 ) maxcount ) ”
+  &&  (store_string str_pre input ))
+  ||
+  (“ (n = (string_length (input))) ” 
+  &&  “ (0 <= i) ” 
+  &&  “ (i < n) ” 
+  &&  “ (0 <= (count - 1 )) ” 
+  &&  “ ((count - 1 ) <= maxcount) ” 
+  &&  “ (maxcount <= (i + 1 )) ” 
+  &&  “ ((Znth i (c_string (input)) 0) = 91) ” 
+  &&  “ (valid_string input ) ” 
+  &&  “ (problem_132_pre_z input ) ” 
+  &&  “ (bracket_codes_z_132 input ) ” 
+  &&  “ ((string_length (input)) < INT_MAX) ” 
+  &&  “ (nested_scan_after_132 input (i + 1 ) (count - 1 ) maxcount ) ”
+  &&  (store_string str_pre input ))
+.
+
+Definition is_nested_entail_wit_2_4 := 
+forall (str_pre: Z) (input: (@list Z)) (ch: Z) (maxcount: Z) (count: Z) (i: Z) (n: Z) (PreH1 : (0 <= maxcount)) (PreH2 : ((count - 1 ) < 0)) (PreH3 : ((Znth i (c_string (input)) 0) = 93)) (PreH4 : ((Znth i (c_string (input)) 0) <> 91)) (PreH5 : (i < n)) (PreH6 : (n = (string_length (input)))) (PreH7 : (0 <= i)) (PreH8 : (i <= n)) (PreH9 : (0 <= count)) (PreH10 : (count <= maxcount)) (PreH11 : (maxcount <= i)) (PreH12 : (0 <= ch)) (PreH13 : (ch <= 127)) (PreH14 : (valid_string input )) (PreH15 : (problem_132_pre_z input )) (PreH16 : (bracket_codes_z_132 input )) (PreH17 : ((string_length (input)) < INT_MAX)) (PreH18 : (nested_scan_state_132 input i count maxcount )) ,
+  (store_string str_pre input )
+|--
+  (“ (n = (string_length (input))) ” 
+  &&  “ (0 <= i) ” 
+  &&  “ (i < n) ” 
+  &&  “ (0 <= 0) ” 
+  &&  “ (0 <= maxcount) ” 
+  &&  “ (maxcount <= (i + 1 )) ” 
+  &&  “ ((Znth i (c_string (input)) 0) = 93) ” 
+  &&  “ (valid_string input ) ” 
+  &&  “ (problem_132_pre_z input ) ” 
+  &&  “ (bracket_codes_z_132 input ) ” 
+  &&  “ ((string_length (input)) < INT_MAX) ” 
+  &&  “ (nested_scan_after_132 input (i + 1 ) 0 maxcount ) ”
+  &&  (store_string str_pre input ))
+  ||
+  (“ (n = (string_length (input))) ” 
+  &&  “ (0 <= i) ” 
+  &&  “ (i < n) ” 
+  &&  “ (0 <= 0) ” 
+  &&  “ (0 <= maxcount) ” 
+  &&  “ (maxcount <= (i + 1 )) ” 
+  &&  “ ((Znth i (c_string (input)) 0) = 91) ” 
+  &&  “ (valid_string input ) ” 
+  &&  “ (problem_132_pre_z input ) ” 
+  &&  “ (bracket_codes_z_132 input ) ” 
+  &&  “ ((string_length (input)) < INT_MAX) ” 
+  &&  “ (nested_scan_after_132 input (i + 1 ) 0 maxcount ) ”
+  &&  (store_string str_pre input ))
+.
+
+Definition is_nested_entail_wit_2_5 := 
+forall (str_pre: Z) (input: (@list Z)) (ch: Z) (maxcount: Z) (count: Z) (i: Z) (n: Z) (PreH1 : ((count + 1 ) > maxcount)) (PreH2 : ((count + 1 ) >= 0)) (PreH3 : ((Znth i (c_string (input)) 0) <> 93)) (PreH4 : ((Znth i (c_string (input)) 0) = 91)) (PreH5 : (i < n)) (PreH6 : (n = (string_length (input)))) (PreH7 : (0 <= i)) (PreH8 : (i <= n)) (PreH9 : (0 <= count)) (PreH10 : (count <= maxcount)) (PreH11 : (maxcount <= i)) (PreH12 : (0 <= ch)) (PreH13 : (ch <= 127)) (PreH14 : (valid_string input )) (PreH15 : (problem_132_pre_z input )) (PreH16 : (bracket_codes_z_132 input )) (PreH17 : ((string_length (input)) < INT_MAX)) (PreH18 : (nested_scan_state_132 input i count maxcount )) ,
+  (store_string str_pre input )
+|--
+  (“ (n = (string_length (input))) ” 
+  &&  “ (0 <= i) ” 
+  &&  “ (i < n) ” 
+  &&  “ (0 <= (count + 1 )) ” 
+  &&  “ ((count + 1 ) <= (count + 1 )) ” 
+  &&  “ ((count + 1 ) <= (i + 1 )) ” 
+  &&  “ ((Znth i (c_string (input)) 0) = 93) ” 
+  &&  “ (valid_string input ) ” 
+  &&  “ (problem_132_pre_z input ) ” 
+  &&  “ (bracket_codes_z_132 input ) ” 
+  &&  “ ((string_length (input)) < INT_MAX) ” 
+  &&  “ (nested_scan_after_132 input (i + 1 ) (count + 1 ) (count + 1 ) ) ”
+  &&  (store_string str_pre input ))
+  ||
+  (“ (n = (string_length (input))) ” 
+  &&  “ (0 <= i) ” 
+  &&  “ (i < n) ” 
+  &&  “ (0 <= (count + 1 )) ” 
+  &&  “ ((count + 1 ) <= (count + 1 )) ” 
+  &&  “ ((count + 1 ) <= (i + 1 )) ” 
+  &&  “ ((Znth i (c_string (input)) 0) = 91) ” 
+  &&  “ (valid_string input ) ” 
+  &&  “ (problem_132_pre_z input ) ” 
+  &&  “ (bracket_codes_z_132 input ) ” 
+  &&  “ ((string_length (input)) < INT_MAX) ” 
+  &&  “ (nested_scan_after_132 input (i + 1 ) (count + 1 ) (count + 1 ) ) ”
+  &&  (store_string str_pre input ))
+.
+
+Definition is_nested_entail_wit_3_1 := 
+(
+forall (str_pre: Z) (input: (@list Z)) (n: Z) (i: Z) (count: Z) (maxcount: Z) (ch: Z) (PreH1 : (count <= (maxcount - 2 ))) (PreH2 : (n = (string_length (input)))) (PreH3 : (0 <= i)) (PreH4 : (i < n)) (PreH5 : (0 <= count)) (PreH6 : (count <= maxcount)) (PreH7 : (maxcount <= (i + 1 ))) (PreH8 : (ch = 91)) (PreH9 : (valid_string input )) (PreH10 : (problem_132_pre_z input )) (PreH11 : (bracket_codes_z_132 input )) (PreH12 : ((string_length (input)) < INT_MAX)) (PreH13 : (nested_scan_after_132 input (i + 1 ) count maxcount )) ,
+  (store_string str_pre input )
+|--
+  “ (problem_132_result_z input 1 ) ”
+  &&  (store_string str_pre input )
+) \/
+(
+forall (input: (@list Z)) (n: Z) (i: Z) (count: Z) (maxcount: Z) (ch: Z) (PreH1 : (0 <= ((string_length (input)) + 1 ))) (PreH2 : (count <= (maxcount - 2 ))) (PreH3 : (n = (string_length (input)))) (PreH4 : (0 <= i)) (PreH5 : (i < n)) (PreH6 : (0 <= count)) (PreH7 : (count <= maxcount)) (PreH8 : (maxcount <= (i + 1 ))) (PreH9 : (ch = 91)) (PreH10 : (valid_string input )) (PreH11 : (problem_132_pre_z input )) (PreH12 : (bracket_codes_z_132 input )) (PreH13 : ((string_length (input)) < INT_MAX)) (PreH14 : (nested_scan_after_132 input (i + 1 ) count maxcount )) ,
+  TT && emp 
+|--
+  “ (problem_132_result_z input 1 ) ”
+  &&  emp
+).
+
+Definition is_nested_entail_wit_3_1_split_goal_1 := 
+forall (input: (@list Z)) (n: Z) (i: Z) (count: Z) (maxcount: Z) (ch: Z) (PreH1 : (0 <= ((string_length (input)) + 1 ))) (PreH2 : (count <= (maxcount - 2 ))) (PreH3 : (n = (string_length (input)))) (PreH4 : (0 <= i)) (PreH5 : (i < n)) (PreH6 : (0 <= count)) (PreH7 : (count <= maxcount)) (PreH8 : (maxcount <= (i + 1 ))) (PreH9 : (ch = 91)) (PreH10 : (valid_string input )) (PreH11 : (problem_132_pre_z input )) (PreH12 : (bracket_codes_z_132 input )) (PreH13 : ((string_length (input)) < INT_MAX)) (PreH14 : (nested_scan_after_132 input (i + 1 ) count maxcount )) ,
+  TT && emp 
+|--
+  “ (problem_132_result_z input 1 ) ”
+.
+
+Definition is_nested_entail_wit_3_2 := 
+(
+forall (str_pre: Z) (input: (@list Z)) (n: Z) (i: Z) (count: Z) (maxcount: Z) (ch: Z) (PreH1 : (count <= (maxcount - 2 ))) (PreH2 : (n = (string_length (input)))) (PreH3 : (0 <= i)) (PreH4 : (i < n)) (PreH5 : (0 <= count)) (PreH6 : (count <= maxcount)) (PreH7 : (maxcount <= (i + 1 ))) (PreH8 : (ch = 93)) (PreH9 : (valid_string input )) (PreH10 : (problem_132_pre_z input )) (PreH11 : (bracket_codes_z_132 input )) (PreH12 : ((string_length (input)) < INT_MAX)) (PreH13 : (nested_scan_after_132 input (i + 1 ) count maxcount )) ,
+  (store_string str_pre input )
+|--
+  “ (problem_132_result_z input 1 ) ”
+  &&  (store_string str_pre input )
+) \/
+(
+forall (input: (@list Z)) (n: Z) (i: Z) (count: Z) (maxcount: Z) (ch: Z) (PreH1 : (0 <= ((string_length (input)) + 1 ))) (PreH2 : (count <= (maxcount - 2 ))) (PreH3 : (n = (string_length (input)))) (PreH4 : (0 <= i)) (PreH5 : (i < n)) (PreH6 : (0 <= count)) (PreH7 : (count <= maxcount)) (PreH8 : (maxcount <= (i + 1 ))) (PreH9 : (ch = 93)) (PreH10 : (valid_string input )) (PreH11 : (problem_132_pre_z input )) (PreH12 : (bracket_codes_z_132 input )) (PreH13 : ((string_length (input)) < INT_MAX)) (PreH14 : (nested_scan_after_132 input (i + 1 ) count maxcount )) ,
+  TT && emp 
+|--
+  “ (problem_132_result_z input 1 ) ”
+  &&  emp
+).
+
+Definition is_nested_entail_wit_3_2_split_goal_1 := 
+forall (input: (@list Z)) (n: Z) (i: Z) (count: Z) (maxcount: Z) (ch: Z) (PreH1 : (0 <= ((string_length (input)) + 1 ))) (PreH2 : (count <= (maxcount - 2 ))) (PreH3 : (n = (string_length (input)))) (PreH4 : (0 <= i)) (PreH5 : (i < n)) (PreH6 : (0 <= count)) (PreH7 : (count <= maxcount)) (PreH8 : (maxcount <= (i + 1 ))) (PreH9 : (ch = 93)) (PreH10 : (valid_string input )) (PreH11 : (problem_132_pre_z input )) (PreH12 : (bracket_codes_z_132 input )) (PreH13 : ((string_length (input)) < INT_MAX)) (PreH14 : (nested_scan_after_132 input (i + 1 ) count maxcount )) ,
+  TT && emp 
+|--
+  “ (problem_132_result_z input 1 ) ”
+.
+
+Definition is_nested_entail_wit_4_1 := 
+(
+forall (str_pre: Z) (input: (@list Z)) (n: Z) (i: Z) (count: Z) (maxcount: Z) (ch: Z) (PreH1 : (count > (maxcount - 2 ))) (PreH2 : (n = (string_length (input)))) (PreH3 : (0 <= i)) (PreH4 : (i < n)) (PreH5 : (0 <= count)) (PreH6 : (count <= maxcount)) (PreH7 : (maxcount <= (i + 1 ))) (PreH8 : (ch = 93)) (PreH9 : (valid_string input )) (PreH10 : (problem_132_pre_z input )) (PreH11 : (bracket_codes_z_132 input )) (PreH12 : ((string_length (input)) < INT_MAX)) (PreH13 : (nested_scan_after_132 input (i + 1 ) count maxcount )) ,
+  (store_string str_pre input )
+|--
+  “ (n = (string_length (input))) ” 
+  &&  “ (0 <= (i + 1 )) ” 
+  &&  “ ((i + 1 ) <= n) ” 
+  &&  “ (0 <= count) ” 
+  &&  “ (count <= maxcount) ” 
+  &&  “ (maxcount <= (i + 1 )) ” 
+  &&  “ (0 <= ch) ” 
+  &&  “ (ch <= 127) ” 
+  &&  “ (valid_string input ) ” 
+  &&  “ (problem_132_pre_z input ) ” 
+  &&  “ (bracket_codes_z_132 input ) ” 
+  &&  “ ((string_length (input)) < INT_MAX) ” 
+  &&  “ (nested_scan_state_132 input (i + 1 ) count maxcount ) ”
+  &&  (store_string str_pre input )
+) \/
+(
+forall (input: (@list Z)) (n: Z) (i: Z) (count: Z) (maxcount: Z) (ch: Z) (PreH1 : (0 <= ((string_length (input)) + 1 ))) (PreH2 : (count > (maxcount - 2 ))) (PreH3 : (n = (string_length (input)))) (PreH4 : (0 <= i)) (PreH5 : (i < n)) (PreH6 : (0 <= count)) (PreH7 : (count <= maxcount)) (PreH8 : (maxcount <= (i + 1 ))) (PreH9 : (ch = 93)) (PreH10 : (valid_string input )) (PreH11 : (problem_132_pre_z input )) (PreH12 : (bracket_codes_z_132 input )) (PreH13 : ((string_length (input)) < INT_MAX)) (PreH14 : (nested_scan_after_132 input (i + 1 ) count maxcount )) ,
+  TT && emp 
+|--
+  “ (nested_scan_state_132 input (i + 1 ) count maxcount ) ”
+  &&  emp
+).
+
+Definition is_nested_entail_wit_4_1_split_goal_1 := 
+forall (input: (@list Z)) (n: Z) (i: Z) (count: Z) (maxcount: Z) (ch: Z) (PreH1 : (0 <= ((string_length (input)) + 1 ))) (PreH2 : (count > (maxcount - 2 ))) (PreH3 : (n = (string_length (input)))) (PreH4 : (0 <= i)) (PreH5 : (i < n)) (PreH6 : (0 <= count)) (PreH7 : (count <= maxcount)) (PreH8 : (maxcount <= (i + 1 ))) (PreH9 : (ch = 93)) (PreH10 : (valid_string input )) (PreH11 : (problem_132_pre_z input )) (PreH12 : (bracket_codes_z_132 input )) (PreH13 : ((string_length (input)) < INT_MAX)) (PreH14 : (nested_scan_after_132 input (i + 1 ) count maxcount )) ,
+  TT && emp 
+|--
+  “ (nested_scan_state_132 input (i + 1 ) count maxcount ) ”
+.
+
+Definition is_nested_entail_wit_4_2 := 
+(
+forall (str_pre: Z) (input: (@list Z)) (n: Z) (i: Z) (count: Z) (maxcount: Z) (ch: Z) (PreH1 : (count > (maxcount - 2 ))) (PreH2 : (n = (string_length (input)))) (PreH3 : (0 <= i)) (PreH4 : (i < n)) (PreH5 : (0 <= count)) (PreH6 : (count <= maxcount)) (PreH7 : (maxcount <= (i + 1 ))) (PreH8 : (ch = 91)) (PreH9 : (valid_string input )) (PreH10 : (problem_132_pre_z input )) (PreH11 : (bracket_codes_z_132 input )) (PreH12 : ((string_length (input)) < INT_MAX)) (PreH13 : (nested_scan_after_132 input (i + 1 ) count maxcount )) ,
+  (store_string str_pre input )
+|--
+  “ (n = (string_length (input))) ” 
+  &&  “ (0 <= (i + 1 )) ” 
+  &&  “ ((i + 1 ) <= n) ” 
+  &&  “ (0 <= count) ” 
+  &&  “ (count <= maxcount) ” 
+  &&  “ (maxcount <= (i + 1 )) ” 
+  &&  “ (0 <= ch) ” 
+  &&  “ (ch <= 127) ” 
+  &&  “ (valid_string input ) ” 
+  &&  “ (problem_132_pre_z input ) ” 
+  &&  “ (bracket_codes_z_132 input ) ” 
+  &&  “ ((string_length (input)) < INT_MAX) ” 
+  &&  “ (nested_scan_state_132 input (i + 1 ) count maxcount ) ”
+  &&  (store_string str_pre input )
+) \/
+(
+forall (input: (@list Z)) (n: Z) (i: Z) (count: Z) (maxcount: Z) (ch: Z) (PreH1 : (0 <= ((string_length (input)) + 1 ))) (PreH2 : (count > (maxcount - 2 ))) (PreH3 : (n = (string_length (input)))) (PreH4 : (0 <= i)) (PreH5 : (i < n)) (PreH6 : (0 <= count)) (PreH7 : (count <= maxcount)) (PreH8 : (maxcount <= (i + 1 ))) (PreH9 : (ch = 91)) (PreH10 : (valid_string input )) (PreH11 : (problem_132_pre_z input )) (PreH12 : (bracket_codes_z_132 input )) (PreH13 : ((string_length (input)) < INT_MAX)) (PreH14 : (nested_scan_after_132 input (i + 1 ) count maxcount )) ,
+  TT && emp 
+|--
+  “ (nested_scan_state_132 input (i + 1 ) count maxcount ) ”
+  &&  emp
+).
+
+Definition is_nested_entail_wit_4_2_split_goal_1 := 
+forall (input: (@list Z)) (n: Z) (i: Z) (count: Z) (maxcount: Z) (ch: Z) (PreH1 : (0 <= ((string_length (input)) + 1 ))) (PreH2 : (count > (maxcount - 2 ))) (PreH3 : (n = (string_length (input)))) (PreH4 : (0 <= i)) (PreH5 : (i < n)) (PreH6 : (0 <= count)) (PreH7 : (count <= maxcount)) (PreH8 : (maxcount <= (i + 1 ))) (PreH9 : (ch = 91)) (PreH10 : (valid_string input )) (PreH11 : (problem_132_pre_z input )) (PreH12 : (bracket_codes_z_132 input )) (PreH13 : ((string_length (input)) < INT_MAX)) (PreH14 : (nested_scan_after_132 input (i + 1 ) count maxcount )) ,
+  TT && emp 
+|--
+  “ (nested_scan_state_132 input (i + 1 ) count maxcount ) ”
+.
+
+Definition is_nested_entail_wit_5 := 
+(
+forall (str_pre: Z) (input: (@list Z)) (ch: Z) (maxcount: Z) (count: Z) (i: Z) (n: Z) (PreH1 : (i >= n)) (PreH2 : (n = (string_length (input)))) (PreH3 : (0 <= i)) (PreH4 : (i <= n)) (PreH5 : (0 <= count)) (PreH6 : (count <= maxcount)) (PreH7 : (maxcount <= i)) (PreH8 : (0 <= ch)) (PreH9 : (ch <= 127)) (PreH10 : (valid_string input )) (PreH11 : (problem_132_pre_z input )) (PreH12 : (bracket_codes_z_132 input )) (PreH13 : ((string_length (input)) < INT_MAX)) (PreH14 : (nested_scan_state_132 input i count maxcount )) ,
+  (store_string str_pre input )
+|--
+  “ (problem_132_result_z input 0 ) ”
+  &&  (store_string str_pre input )
+) \/
+(
+forall (input: (@list Z)) (ch: Z) (maxcount: Z) (count: Z) (i: Z) (n: Z) (PreH1 : (0 <= ((string_length (input)) + 1 ))) (PreH2 : (i >= n)) (PreH3 : (n = (string_length (input)))) (PreH4 : (0 <= i)) (PreH5 : (i <= n)) (PreH6 : (0 <= count)) (PreH7 : (count <= maxcount)) (PreH8 : (maxcount <= i)) (PreH9 : (0 <= ch)) (PreH10 : (ch <= 127)) (PreH11 : (valid_string input )) (PreH12 : (problem_132_pre_z input )) (PreH13 : (bracket_codes_z_132 input )) (PreH14 : ((string_length (input)) < INT_MAX)) (PreH15 : (nested_scan_state_132 input i count maxcount )) ,
+  TT && emp 
+|--
+  “ (problem_132_result_z input 0 ) ”
+  &&  emp
+).
+
+Definition is_nested_entail_wit_5_split_goal_1 := 
+forall (input: (@list Z)) (ch: Z) (maxcount: Z) (count: Z) (i: Z) (n: Z) (PreH1 : (0 <= ((string_length (input)) + 1 ))) (PreH2 : (i >= n)) (PreH3 : (n = (string_length (input)))) (PreH4 : (0 <= i)) (PreH5 : (i <= n)) (PreH6 : (0 <= count)) (PreH7 : (count <= maxcount)) (PreH8 : (maxcount <= i)) (PreH9 : (0 <= ch)) (PreH10 : (ch <= 127)) (PreH11 : (valid_string input )) (PreH12 : (problem_132_pre_z input )) (PreH13 : (bracket_codes_z_132 input )) (PreH14 : ((string_length (input)) < INT_MAX)) (PreH15 : (nested_scan_state_132 input i count maxcount )) ,
+  TT && emp 
+|--
+  “ (problem_132_result_z input 0 ) ”
+.
+
+Definition is_nested_return_wit_1 := 
+forall (str_pre: Z) (input: (@list Z)) (PreH1 : (problem_132_result_z input 0 )) ,
+  (store_string str_pre input )
+|--
+  “ (problem_132_result_z input 0 ) ”
+  &&  (store_string str_pre input )
+.
+
+Definition is_nested_return_wit_2 := 
+forall (str_pre: Z) (input: (@list Z)) (PreH1 : (problem_132_result_z input 1 )) ,
+  (store_string str_pre input )
+|--
+  “ (problem_132_result_z input 1 ) ”
+  &&  (store_string str_pre input )
+.
+
+Definition is_nested_partial_solve_wit_1_pure := 
+forall (str_pre: Z) (input: (@list Z)) (PreH1 : (valid_string input )) (PreH2 : (problem_132_pre_z input )) (PreH3 : (bracket_codes_z_132 input )) (PreH4 : ((string_length (input)) < INT_MAX)) ,
+  ((( &( "n" ) )) # Int  |->_)
+  **  ((( &( "str" ) )) # Ptr  |-> str_pre)
+  **  (store_string str_pre input )
+|--
+  “ (valid_string input ) ” 
+  &&  “ ((string_length (input)) < INT_MAX) ”
+.
+
+Definition is_nested_partial_solve_wit_1_aux := 
+forall (str_pre: Z) (input: (@list Z)) (PreH1 : (valid_string input )) (PreH2 : (problem_132_pre_z input )) (PreH3 : (bracket_codes_z_132 input )) (PreH4 : ((string_length (input)) < INT_MAX)) ,
+  (store_string str_pre input )
+|--
+  “ (valid_string input ) ” 
+  &&  “ ((string_length (input)) < INT_MAX) ” 
+  &&  “ (0 <= ((string_length (input)) + 1 )) ” 
+  &&  “ (valid_string input ) ” 
+  &&  “ (problem_132_pre_z input ) ” 
+  &&  “ (bracket_codes_z_132 input ) ” 
+  &&  “ ((string_length (input)) < INT_MAX) ”
+  &&  (store_string str_pre input )
+.
+
+Definition is_nested_partial_solve_wit_1 := is_nested_partial_solve_wit_1_pure -> is_nested_partial_solve_wit_1_aux.
+
+Module Type VC_Correct.
+
+Include char_array_Strategy_Correct.
+Include string_Strategy_Correct.
+
+Axiom proof_of_is_nested_safety_wit_1 : is_nested_safety_wit_1.
+Axiom proof_of_is_nested_safety_wit_2 : is_nested_safety_wit_2.
+Axiom proof_of_is_nested_safety_wit_3 : is_nested_safety_wit_3.
+Axiom proof_of_is_nested_safety_wit_4 : is_nested_safety_wit_4.
+Axiom proof_of_is_nested_safety_wit_5 : is_nested_safety_wit_5.
+Axiom proof_of_is_nested_safety_wit_6 : is_nested_safety_wit_6.
+Axiom proof_of_is_nested_safety_wit_7 : is_nested_safety_wit_7.
+Axiom proof_of_is_nested_safety_wit_8 : is_nested_safety_wit_8.
+Axiom proof_of_is_nested_safety_wit_9 : is_nested_safety_wit_9.
+Axiom proof_of_is_nested_safety_wit_10 : is_nested_safety_wit_10.
+Axiom proof_of_is_nested_safety_wit_11 : is_nested_safety_wit_11.
+Axiom proof_of_is_nested_safety_wit_12 : is_nested_safety_wit_12.
+Axiom proof_of_is_nested_safety_wit_13 : is_nested_safety_wit_13.
+Axiom proof_of_is_nested_safety_wit_14 : is_nested_safety_wit_14.
+Axiom proof_of_is_nested_safety_wit_15 : is_nested_safety_wit_15.
+Axiom proof_of_is_nested_safety_wit_16 : is_nested_safety_wit_16.
+Axiom proof_of_is_nested_safety_wit_17 : is_nested_safety_wit_17.
+Axiom proof_of_is_nested_safety_wit_18 : is_nested_safety_wit_18.
+Axiom proof_of_is_nested_safety_wit_19 : is_nested_safety_wit_19.
+Axiom proof_of_is_nested_safety_wit_20 : is_nested_safety_wit_20.
+Axiom proof_of_is_nested_safety_wit_21 : is_nested_safety_wit_21.
+Axiom proof_of_is_nested_safety_wit_22 : is_nested_safety_wit_22.
+Axiom proof_of_is_nested_safety_wit_23 : is_nested_safety_wit_23.
+Axiom proof_of_is_nested_safety_wit_24 : is_nested_safety_wit_24.
+Axiom proof_of_is_nested_safety_wit_25 : is_nested_safety_wit_25.
+Axiom proof_of_is_nested_safety_wit_26 : is_nested_safety_wit_26.
+Axiom proof_of_is_nested_safety_wit_27 : is_nested_safety_wit_27.
+Axiom proof_of_is_nested_safety_wit_28 : is_nested_safety_wit_28.
+Axiom proof_of_is_nested_safety_wit_29 : is_nested_safety_wit_29.
+Axiom proof_of_is_nested_entail_wit_1 : is_nested_entail_wit_1.
+Axiom proof_of_is_nested_entail_wit_2_1 : is_nested_entail_wit_2_1.
+Axiom proof_of_is_nested_entail_wit_2_2 : is_nested_entail_wit_2_2.
+Axiom proof_of_is_nested_entail_wit_2_3 : is_nested_entail_wit_2_3.
+Axiom proof_of_is_nested_entail_wit_2_4 : is_nested_entail_wit_2_4.
+Axiom proof_of_is_nested_entail_wit_2_5 : is_nested_entail_wit_2_5.
+Axiom proof_of_is_nested_entail_wit_3_1 : is_nested_entail_wit_3_1.
+Axiom proof_of_is_nested_entail_wit_3_2 : is_nested_entail_wit_3_2.
+Axiom proof_of_is_nested_entail_wit_4_1 : is_nested_entail_wit_4_1.
+Axiom proof_of_is_nested_entail_wit_4_2 : is_nested_entail_wit_4_2.
+Axiom proof_of_is_nested_entail_wit_5 : is_nested_entail_wit_5.
+Axiom proof_of_is_nested_return_wit_1 : is_nested_return_wit_1.
+Axiom proof_of_is_nested_return_wit_2 : is_nested_return_wit_2.
+Axiom proof_of_is_nested_partial_solve_wit_1_pure : is_nested_partial_solve_wit_1_pure.
+Axiom proof_of_is_nested_partial_solve_wit_1 : is_nested_partial_solve_wit_1.
+
+End VC_Correct.
