QCP_examples/humaneval/spec_logic_rewrite_c_files/coins_132.v
@@ -1,0 +1,276 @@
+Load "../spec/132".
+
+Require Import Coq.ZArith.ZArith.
+Require Import Coq.Bool.Bool.
+Require Import Coq.Lists.List.
+Require Import Coq.Strings.String.
+Require Import Coq.Strings.Ascii.
+Require Import Lia.
+From AUXLib Require Import ListLib.
+Require Import SimpleC.StdLib.string_lib.
+
+Import ListNotations.
+Local Open Scope Z_scope.
+Local Open Scope string_scope.
+Local Open Scope list_scope.
+
+Definition ascii_of_z_132 (z : Z) : ascii :=
+  ascii_of_nat (Z.to_nat z).
+
+Fixpoint string_of_list_z_132 (l : list Z) : string :=
+  match l with
+  | [] => EmptyString
+  | c :: rest => String (ascii_of_z_132 c) (string_of_list_z_132 rest)
+  end.
+
+Definition string_length (l : list Z) : Z := Zlength l.
+
+Definition problem_132_pre_z (l : list Z) : Prop :=
+  problem_132_pre (string_of_list_z_132 l).
+
+Definition problem_132_spec_z (l : list Z) (output : bool) : Prop :=
+  problem_132_spec (string_of_list_z_132 l) output.
+
+Definition problem_132_result_z (l : list Z) (output : Z) : Prop :=
+  problem_132_spec_z l (Z.eqb output 1).
+
+Definition bracket_codes_z_132 (l : list Z) : Prop :=
+  Forall (fun c => c = 91 \/ c = 93) l.
+
+Definition initial_bracket_scan_132 : bracket_scan_state :=
+  {| scan_current := 0; scan_maximum := 0; scan_nested := false |}.
+
+Definition scan_prefix_132 (input : list Z) (i : Z) : bracket_scan_state :=
+  fold_left bracket_scan_step
+    (map ascii_of_z_132 (sublist 0 i input))
+    initial_bracket_scan_132.
+
+Definition nested_scan_state_132
+    (input : list Z) (i count maximum : Z) : Prop :=
+  0 <= i <= Zlength input /\
+  count = scan_current (scan_prefix_132 input i) /\
+  maximum = scan_maximum (scan_prefix_132 input i) /\
+  scan_nested (scan_prefix_132 input i) = false.
+
+Definition nested_scan_after_132
+    (input : list Z) (i count maximum : Z) : Prop :=
+  0 <= i <= Zlength input /\
+  count = scan_current (scan_prefix_132 input i) /\
+  maximum = scan_maximum (scan_prefix_132 input i) /\
+  scan_nested (scan_prefix_132 input i) = Z.leb (count + 2) maximum.
+
+Lemma list_ascii_string_of_list_z_132 : forall l,
+  list_ascii_of_string (string_of_list_z_132 l) = map ascii_of_z_132 l.
+Proof.
+  induction l as [|c rest IH]; simpl; [reflexivity|].
+  now rewrite IH.
+Qed.
+
+Lemma ascii_of_z_open_132 : ascii_of_z_132 91 = open_bracket.
+Proof. vm_compute. reflexivity. Qed.
+
+Lemma ascii_of_z_close_132 : ascii_of_z_132 93 = close_bracket.
+Proof. vm_compute. reflexivity. Qed.
+
+Lemma nat_of_ascii_ascii_of_z_132 : forall z,
+  0 <= z < 256 ->
+  nat_of_ascii (ascii_of_z_132 z) = Z.to_nat z.
+Proof.
+  intros z Hz.
+  unfold ascii_of_z_132.
+  rewrite nat_ascii_embedding by lia.
+  reflexivity.
+Qed.
+
+Lemma problem_132_pre_valid_bracket_codes : forall input,
+  problem_132_pre_z input ->
+  valid_string input ->
+  bracket_codes_z_132 input.
+Proof.
+  intros input Hpre [Hrange _].
+  unfold problem_132_pre_z, problem_132_pre in Hpre.
+  rewrite list_ascii_string_of_list_z_132 in Hpre.
+  unfold bracket_codes_z_132.
+  apply Forall_forall.
+  intros z Hin.
+  apply Forall_forall with (x := ascii_of_z_132 z) in Hpre.
+  - destruct (In_nth input z 0 Hin) as [n [Hn Hnth]].
+    assert (Hzrange : 0 <= z <= 127).
+    { specialize (Hrange (Z.of_nat n)).
+      assert (0 <= Z.of_nat n < Zlength input).
+      { rewrite Zlength_correct; lia. }
+      specialize (Hrange H).
+      unfold Znth in Hrange.
+      rewrite Nat2Z.id in Hrange.
+      now rewrite Hnth in Hrange. }
+    destruct Hpre as [Hopen | Hclose].
+    + left.
+      apply f_equal with (f := nat_of_ascii) in Hopen.
+      rewrite nat_of_ascii_ascii_of_z_132 in Hopen by lia.
+      vm_compute in Hopen.
+      apply Z2Nat.inj; try lia.
+      exact Hopen.
+    + right.
+      apply f_equal with (f := nat_of_ascii) in Hclose.
+      rewrite nat_of_ascii_ascii_of_z_132 in Hclose by lia.
+      vm_compute in Hclose.
+      apply Z2Nat.inj; try lia.
+      exact Hclose.
+  - apply in_map; exact Hin.
+Qed.
+
+Lemma sublist_succ_132 : forall input i,
+  0 <= i < Zlength input ->
+  sublist 0 (i + 1) input = sublist 0 i input ++ [Znth i input 0].
+Proof.
+  intros input i Hi.
+  rewrite (sublist_split 0 (i + 1) i input) by lia.
+  rewrite (sublist_single 0 i input) by lia.
+  reflexivity.
+Qed.
+
+Lemma scan_prefix_succ_132 : forall input i,
+  0 <= i < Zlength input ->
+  scan_prefix_132 input (i + 1) =
+  bracket_scan_step (scan_prefix_132 input i)
+    (ascii_of_z_132 (Znth i input 0)).
+Proof.
+  intros input i Hi.
+  unfold scan_prefix_132.
+  rewrite (sublist_succ_132 input i Hi), map_app.
+  simpl.
+  rewrite fold_left_app.
+  reflexivity.
+Qed.
+
+Lemma bracket_codes_Znth_132 : forall input i,
+  bracket_codes_z_132 input ->
+  0 <= i < Zlength input ->
+  Znth i input 0 = 91 \/ Znth i input 0 = 93.
+Proof.
+  intros input i Hcodes Hi.
+  unfold bracket_codes_z_132 in Hcodes.
+  apply Forall_forall with (x := Znth i input 0) in Hcodes.
+  - exact Hcodes.
+  - unfold Znth.
+    apply nth_In.
+    rewrite Zlength_correct in Hi.
+    lia.
+Qed.
+
+Lemma nested_scan_initial_132 : forall input,
+  nested_scan_state_132 input 0 0 0.
+Proof.
+  intros input.
+  unfold nested_scan_state_132, scan_prefix_132,
+    initial_bracket_scan_132.
+  simpl.
+  split; [pose proof (Zlength_nonneg input); lia|].
+  repeat split; reflexivity.
+Qed.
+
+Lemma nested_scan_step_132 : forall input i count maximum ch count' maximum',
+  nested_scan_state_132 input i count maximum ->
+  i < Zlength input ->
+  ch = Znth i input 0 ->
+  (ch = 91 \/ ch = 93) ->
+  count' = (if Z.eqb ch 91 then count + 1 else Z.max 0 (count - 1)) ->
+  maximum' = Z.max maximum count' ->
+  nested_scan_after_132 input (i + 1) count' maximum'.
+Proof.
+  intros input i count maximum ch count' maximum'
+    Hstate Hi Hch Hcodes Hcount Hmaximum.
+  unfold nested_scan_state_132 in Hstate.
+  destruct Hstate as [Hrange [Hcount0 [Hmaximum0 Hfound]]].
+  unfold nested_scan_after_132.
+  rewrite scan_prefix_succ_132 by lia.
+  subst ch count maximum count' maximum'.
+  destruct Hcodes as [Hopen | Hclose].
+  - rewrite Hopen, ascii_of_z_open_132.
+    unfold bracket_scan_step; cbn [scan_current scan_maximum scan_nested].
+    rewrite Hfound; cbn [orb].
+    repeat split; try lia; reflexivity.
+  - rewrite Hclose, ascii_of_z_close_132.
+    unfold bracket_scan_step; cbn [scan_current scan_maximum scan_nested].
+    rewrite Hfound; cbn [orb].
+    repeat split; try lia; reflexivity.
+Qed.
+
+Lemma nested_scan_after_continue_132 : forall input i count maximum,
+  nested_scan_after_132 input i count maximum ->
+  maximum - 2 < count ->
+  nested_scan_state_132 input i count maximum.
+Proof.
+  intros input i count maximum Hafter Hcontinue.
+  unfold nested_scan_after_132 in Hafter.
+  unfold nested_scan_state_132.
+  destruct Hafter as [Hrange [Hcount [Hmaximum Hfound]]].
+  refine (conj Hrange (conj Hcount (conj Hmaximum _))).
+  rewrite Hfound.
+  apply Z.leb_gt; lia.
+Qed.
+
+Lemma scan_nested_step_true_132 : forall state c,
+  scan_nested state = true ->
+  scan_nested (bracket_scan_step state c) = true.
+Proof.
+  intros state c H.
+  unfold bracket_scan_step.
+  destruct (ascii_dec c open_bracket); simpl; now rewrite H.
+Qed.
+
+Lemma scan_nested_fold_true_132 : forall chars state,
+  scan_nested state = true ->
+  scan_nested (fold_left bracket_scan_step chars state) = true.
+Proof.
+  induction chars as [|c rest IH]; intros state H; simpl; [exact H|].
+  apply IH. now apply scan_nested_step_true_132.
+Qed.
+
+Lemma scan_prefix_full_132 : forall input,
+  scan_prefix_132 input (Zlength input) =
+  canonical_bracket_scan (string_of_list_z_132 input).
+Proof.
+  intros input.
+  unfold scan_prefix_132, canonical_bracket_scan,
+    initial_bracket_scan_132.
+  rewrite (sublist_self input (Zlength input) eq_refl),
+    list_ascii_string_of_list_z_132.
+  reflexivity.
+Qed.
+
+Lemma nested_scan_after_found_132 : forall input i count maximum,
+  nested_scan_after_132 input i count maximum ->
+  count <= maximum - 2 ->
+  problem_132_result_z input 1.
+Proof.
+  intros input i count maximum Hafter Hfound.
+  unfold nested_scan_after_132 in Hafter.
+  destruct Hafter as [Hrange [Hcount [Hmaximum Hnested]]].
+  assert (Hprefix : scan_nested (scan_prefix_132 input i) = true).
+  { rewrite Hnested, Z.leb_le; lia. }
+  unfold problem_132_result_z, problem_132_spec_z, problem_132_spec.
+  simpl.
+  split; [intros _|intros _; reflexivity].
+  unfold nested_depth_drop.
+  rewrite <- scan_prefix_full_132.
+  unfold scan_prefix_132 in *.
+  rewrite (sublist_split 0 (Zlength input) i input) by lia.
+  rewrite map_app, fold_left_app.
+  apply scan_nested_fold_true_132; exact Hprefix.
+Qed.
+
+Lemma nested_scan_final_false_132 : forall input count maximum,
+  nested_scan_state_132 input (Zlength input) count maximum ->
+  problem_132_result_z input 0.
+Proof.
+  intros input count maximum Hstate.
+  unfold nested_scan_state_132 in Hstate.
+  destruct Hstate as [_ [_ [_ Hfalse]]].
+  unfold problem_132_result_z, problem_132_spec_z, problem_132_spec.
+  simpl.
+  split; [discriminate|].
+  unfold nested_depth_drop.
+  rewrite <- scan_prefix_full_132.
+  now rewrite Hfalse.
+Qed.
